veric/juicy_mem_lemmas.v
@@ -11,56 +11,6 @@ Section mpred.
 
 Context `{!heapGS Σ}.
 
-(*
-(*Lemma inflate_initial_mem_empty:
-  forall lev, emp (inflate_initial_mem Mem.empty lev).
-intro lev.
-unfold inflate_initial_mem.
-destruct (make_rmap (inflate_initial_mem' Mem.empty lev) (core (ghost_of lev))
-        (inflate_initial_mem'_valid Mem.empty lev) (level lev)
-        (inflate_initial_mem'_fmap Mem.empty lev)); simpl.
-{ rewrite core_ghost_of, <- level_core; apply ghost_of_approx. }
-destruct a.
-apply resource_at_empty2.
-intro l; rewrite H0.
-unfold inflate_initial_mem'.
-destruct l.
-unfold access_at; unfold empty at 1.
-simpl.
-rewrite PMap.gi.
-destruct (max_access_at empty (b,z)); try destruct p; try apply NO_identity.
-Qed.
-Local Hint Resolve inflate_initial_mem_empty : core.*)
-
-(* TODO: move this somewhere more appropriate *)
-Definition no_VALs (phi: rmap) := forall loc,
-  match phi @ loc with
-    | YES _ _ (VAL _) _ => False | _ => True
-  end.
-
-Lemma perm_of_sh_join_sub: forall (sh1 sh2: Share.t) p,
-  perm_of_sh sh1 = Some p ->
-  join_sub sh1 sh2 ->
-  perm_order' (perm_of_sh sh2) p.
-Proof.
-intros.
-destruct H0.
-unfold perm_of_sh in *.
-repeat if_tac in H; inv H.
-+
-inv H0. rewrite Share.glb_commute, Share.glb_top in H; subst x.
- rewrite (Share.lub_bot).
-rewrite if_true by auto. rewrite if_true by auto. constructor.
-+ apply join_writable01 in H0 ;auto. rewrite if_true by auto.
-  if_tac; constructor.
-+ apply join_readable1 in H0; auto.
-  if_tac. if_tac; constructor. rewrite if_true by auto. constructor.
-+ assert (sh2 <> Share.bot). contradict H3.
-  apply split_identity in H0; auto. apply identity_share_bot; auto.
-  subst; auto.
-  repeat if_tac; try constructor. contradiction.
-Qed.*)
-
 Lemma perm_order'_trans: forall p1 p2 p3,
   perm_order' (Some p1) p2 -> perm_order' (Some p2) p3 -> perm_order' (Some p1) p3.
 Proof.
@@ -70,44 +20,6 @@ eapply perm_order_trans; eauto.
 Qed.
 
 (* core load and coherence properties *)
-
-(*Lemma writable_perm:
-  forall b i jm, writable (b,i) (m_phi jm) -> Mem.perm (m_dry jm) b i Cur Writable.
-Proof.
-intros until jm; intros H.
-assert (Hacc := juicy_mem_access jm).
-unfold access_cohere in Hacc.
-unfold Mem.perm, Mem.perm_order'.
-specialize ( Hacc (b, i)).
-simpl in H.
-destruct (m_phi jm @ (b, i)).
-contradiction.
-destruct H as [H1 H2]. destruct k; inv H2.
-unfold access_at in Hacc.
-simpl in Hacc.
-rewrite Hacc.
-clear - H1.
-simpl.
-unfold perm_of_sh. rewrite if_true by auto. if_tac; constructor.
-contradiction.
-Qed.
-
-Lemma valid_access_None: forall m ch b b' ofs ofs' p,
-  Mem.valid_access m ch b ofs p
-  -> adr_range (b, ofs) (size_chunk ch) (b', ofs')
-  -> access_at m (b', ofs') Cur = None
-  -> False.
-Proof.
-unfold access_at, Mem.valid_access, Mem.perm, Mem.range_perm, Mem.perm, Mem.perm_order'.
-simpl.
-intros.
-destruct H as [H ?].
-destruct H0 as [H3 H4].
-subst.
-specialize( H ofs' H4).
-rewrite H1 in H.
-auto.
-Qed.*)
 
 Lemma core_load_coherent: forall ch v b ofs bl m,
   mem_auth m ∗ core_load' ch (b, ofs) v bl ⊢
@@ -191,206 +103,6 @@ Proof.
   iDestruct "H" as "((% & <- & %) & H)"; subst; done.
 Qed.
 
-(*Lemma Zminus_lem: forall z1 z2, z1 <= z2 -> Z.to_nat (z2 - z1) = O -> z1=z2.
-Proof. lia. Qed.
-
-Lemma nat_of_Z_lem1: forall n z, 
-    S n = Z.to_nat z -> n = Z.to_nat (z - 1).
-Proof. lia. Qed.
-
-Lemma nat_of_Z_lem2: forall n z1 z2, S n = Z.to_nat (z1 - z2) -> n = Z.to_nat (z1 - z2 - 1).
-Proof. intros; apply nat_of_Z_lem1; auto. Qed.
-
-Lemma nth_getN: forall m b ofs ofs' z,
-  ofs <= ofs' < ofs + z
-  -> z >= 0
-  -> contents_at m (b, ofs')
-  = nth (Z.to_nat (ofs' - ofs)) (Mem.getN (Z.to_nat z) ofs (PMap.get b (Mem.mem_contents m))) Undef.
-Proof.
-intros.
-revert ofs ofs' H H0.
-remember (Z.to_nat z) as n.
-revert n z Heqn.
-induction n; intros.
-destruct z.
-inv H.
-lia.
-simpl in *.
-generalize (lt_O_nat_of_P p). intro.
-lia.
-generalize (Zlt_neg_0 p).
-intro.
-lia.
-simpl.
-case_eq (Z.to_nat (ofs' - ofs)).
-intros.
-assert (ofs = ofs').
-  destruct H.
-  apply Zminus_lem; auto.
-subst; auto.
-intros.
-symmetry in H1.
-assert (n = Z.to_nat (z - 1)) by (apply nat_of_Z_lem1 in Heqn; auto).
-rewrite (IHn (z - 1) H2 (ofs + 1)); try solve [auto|lia].
-assert (Z.to_nat (ofs' - (ofs + 1)) = n0).
-replace (ofs' - (ofs + 1)) with (ofs' - ofs - 1) by lia.
-  apply nat_of_Z_lem1 in H1.
-  auto.
-rewrite H3; auto.
-Qed.*)
-
-(* When would we need to generate a core_load assertion while already knowing the resources in a state?
-Lemma load_core_load: forall ch b ofs v m,
-  Mem.load ch (m_dry m) b ofs = Some v ->
-  mem_auth m ∗ ([∗ list] z ∈ seq 0 (size_chunk_nat ch), ⌜coherent_loc m 
-
-forall z, ofs <= z < ofs + size_chunk ch ->
-                      perm_order'' (perm_of_res (m_phi m @ (b,z))) (Some Readable)) ->
-   ⊢ mem_auth m ∗ core_load ch (b, ofs) v.
-Proof.
-intros until m; intros H PERM.
-hnf.
-unfold Mem.load in H.
-
-if_tac in H; try solve [inv H].
-inversion H.
-clear H.
-exists (Mem.getN (size_chunk_nat ch) ofs (PMap.get b (Mem.mem_contents (m_dry m)))).
-generalize H0 as H0'; intro.
-Local Hint Resolve Mem.getN_length : core.
-unfold Mem.valid_access in H0'.
-destruct H0' as [H0'1 H0'2].
-repeat split; auto.
-clear H0'1 H0'2.
-intros (b', ofs').
-hnf.
-if_tac; hnf; auto.
-assert (Heqbb': b = b').
-  unfold adr_range in H. decompose [and] H. auto.
-pose proof (juicy_mem_contents m).
-pose proof I. (* pose proof (juicy_mem_access m).*)
-pose proof I.
-pose proof I.
-clear H4. subst b'; clear H5.
-destruct H as [_ ?].
-specialize (PERM ofs' H).
-(*
-unfold access_cohere in H3.
-specialize (H3 (b, ofs').
-*)
-unfold perm_of_res in *.
-destruct H0 as [H0 _].
-specialize (H0 ofs').
-specialize (H0 H).
-hnf in H0.
-(*unfold access_at in H3.
-simpl in H3.
-*)
-destruct ((mem_access (m_dry m)) !! b ofs' Cur); try contradiction.
-destruct (m_phi m @ (b, ofs')) eqn:H8; try contradiction.
-if_tac in PERM; inv PERM.
-destruct k; try now inv PERM.
-pose proof (size_chunk_pos ch).
-rewrite <- nth_getN with (ofs := ofs) (z := size_chunk ch); auto; try lia.
-exists sh, r.
-destruct (H1 _ _ _ _ _ H8); subst.
-f_equal.
-inv PERM.
-Qed.
-
-Lemma core_load_load: forall ch b ofs v m,
-  (forall z, ofs <= z < ofs + size_chunk ch ->
-                      perm_order'' (perm_of_res (m_phi m @ (b,z))) (Some Readable)) ->
-  (core_load ch (b, ofs) v (m_phi m) <-> Mem.load ch (m_dry m) b ofs = Some v).
-Proof.
-intros.
-split; [apply core_load_load'| ].
-intros; apply load_core_load; auto.
-Qed.*)
-
-(*Lemma address_mapsto_exists':
-  forall ch v sh (rsh: readable_share sh) loc m lev,
-      (align_chunk ch | snd loc)
-      -> Mem.load ch m (fst loc) (snd loc) = Some v 
-      -> exists w, address_mapsto ch v sh loc w /\ level w = lev.
-Proof.
-intros. rename H into Halign.
-unfold address_mapsto.
-pose (f l' := if adr_range_dec loc (size_chunk ch) l'
-                     then YES sh rsh (VAL (nthbyte (snd l' - snd loc) (Mem.getN (size_chunk_nat ch) (snd loc) (PMap.get (fst loc) (Mem.mem_contents m))))) NoneP
-                     else NO Share.bot bot_unreadable).
-assert (CompCert_AV.valid (res_option oo f)).
-apply VAL_valid.
-unfold compose, f; intros.
-if_tac in H.
-simpl in H.
-injection H;intros; subst k; auto.
-inv H.
-destruct (make_rmap f H lev) as [phi [? ?]].
-extensionality l; unfold f, compose; simpl.
-if_tac; hnf; auto.
-exists phi.
-split; auto.
-exists (Mem.getN (size_chunk_nat ch) (snd loc) (PMap.get (fst loc) (Mem.mem_contents m))).
-split.
-repeat split; auto.
-Transparent Mem.load.
-unfold load in *. if_tac in H0. injection H0. auto. inv H0.
-intro l'.
-unfold jam.
-hnf.
-simpl.
-rewrite H2; clear H H1 H2.
-unfold f; clear f.
-if_tac.
-exists rsh.
-f_equal. 
-apply NO_identity.
-Qed.*)
-
-(*Lemma mapsto_valid_access: forall ch v sh b ofs m,
-  mem_auth m ∗ address_mapsto ch v sh (b, ofs) ⊢
-  ⌜Mem.valid_access m ch b ofs Readable⌝.
-Proof.
-  Search address_mapsto readable_share.
-core_load_valid
-intros.
-unfold address_mapsto in H.
-unfold Mem.valid_access, Mem.range_perm.
-split.
-destruct H as [x [y [Hjoin ?]]].
-destruct H as [[bl [[H2 [H3 H3']] H]] ?].
-hnf in H.
-intros ofs' H4.
-specialize (H (b, ofs')).
-hnf in H.
-destruct (adr_range_dec (b, ofs) (size_chunk ch) (b, ofs')) as [H5|H5].
-  2: unfold adr_range in H5.
-  2: exfalso; apply H5; split; auto.
-hnf in H.
-destruct H as [pf H].
-hnf in H.
-rewrite preds_fmap_NoneP in H.
-simpl in H.
-generalize (resource_at_join _ _ _ (b,ofs') Hjoin); rewrite H; intro.
-forget ((nth (Z.to_nat (ofs' - ofs)) bl Undef)) as v'.
-assert (exists rsh', exists sh', m_phi jm @ (b,ofs') = YES rsh' sh' (VAL v') NoneP).
-inv H1; eauto.
-destruct H6 as [rsh' [sh' ?]].
-generalize (juicy_mem_access jm (b,ofs')); rewrite H6; unfold perm_of_res; simpl; intro.
-clear - H7 sh'.
-unfold perm, access_at in *.
-simpl in H7.
-forget ((mem_access (m_dry jm)) !! b ofs' Cur) as p1.
-unfold perm_of_sh in H7.
-if_tac in H7.
-if_tac in H7; inv H7; constructor.
-rewrite if_true in H7 by auto.
-subst; constructor.
-repeat match goal with [ H: context[ _ /\ _ ] |- _] => destruct H end.
-auto.
-Qed.*)
-
 Lemma mapsto_coherent: forall ch v sh b ofs m,
   mem_auth m ∗ address_mapsto ch v sh (b, ofs) ⊢
   ⌜∃ bl, length bl = size_chunk_nat ch ∧ decode_val ch bl = v ∧ (align_chunk ch | ofs)%Z ∧ forall i, 0 <= i < size_chunk_nat ch -> coherent_loc m (b, ofs + Z.of_nat i)%Z (DfracOwn (Share sh), Some (VAL (nthbyte i bl)))⌝.
@@ -424,36 +136,6 @@ Proof.
   if_tac; constructor.
 Qed.
 
-(*Search Mem.valid_access Mem.store.
-Program Definition mapsto_can_store_definition ch v sh (wsh: writable0_share sh) b ofs m (v':val)
-  (MAPSTO: (address_mapsto ch v sh (b, ofs) * TT)%pred (m_phi jm)):
-  Memory.mem.
-Proof. intros.
-pose proof (mapsto_valid_access_wr _ _ _ wsh _ _ _ MAPSTO).
-apply (mkmem
-  (PMap.set b (setN (encode_val ch v') ofs (PMap.get b (mem_contents (m_dry jm))))
-    (mem_contents (m_dry jm))) (mem_access (m_dry jm))
-  (nextblock (m_dry jm)) (access_max (m_dry jm)) (nextblock_noaccess (m_dry jm))).
-intros. destruct jm; simpl.
-  rewrite PMap.gsspec. destruct (peq b0 b).
-  rewrite setN_default. apply contents_default.
-  apply contents_default.
-Defined.
-
-Lemma mapsto_can_store_property: forall (ch:memory_chunk) v sh (wsh: writable0_share sh) b ofs jm v'
-  (MAPSTO: (address_mapsto ch v sh (b, ofs) * TT)%pred (m_phi jm)),
-  Mem.store ch (m_dry jm) b ofs v' = 
-  Some(mapsto_can_store_definition _ _ _ wsh _ _ jm v' MAPSTO).
-Proof.
-intros.
-pose proof (mapsto_valid_access_wr _ _ _ wsh _ _ _ MAPSTO).
-unfold mapsto_can_store_definition. simpl.
-Transparent Mem.store. unfold store.
-destruct (valid_access_dec (m_dry jm) ch b ofs Writable).
-f_equal. f_equal; auto with extensionality.
-contradiction.
-Opaque Mem.store.
-Qed.*)
 
 Lemma mapsto_can_store: forall ch v sh (wsh: writable0_share sh) b ofs m v',
   mem_auth m ∗ address_mapsto ch v sh (b, ofs) ⊢
@@ -716,14 +398,13 @@ Proof.
   iSplit; iIntros "[-> ?]"; iFrame; done.
 Qed.
 
-Lemma VALspec_range_can_free: forall m n l,
-  mem_auth m ∗ VALspec_range n Share.top l ⊢
-  ⌜∃ m', free m l.1 l.2 (l.2 + n) = Some m'⌝.
+Lemma VALspec_range_perm: forall m n sh l p, perm_of_sh sh = Some p ->
+  mem_auth m ∗ VALspec_range n sh l ⊢
+  ⌜Mem.range_perm m l.1 l.2 (l.2 + n) Cur p⌝.
 Proof.
   intros.
   iIntros "(Hm & H)".
-  iAssert ⌜range_perm m l.1 l.2 (l.2 + n) Cur Freeable⌝ as %H; last by iPureIntro; apply range_perm_free in H as [??]; eauto.
-  iIntros (??).
+  iIntros (a ?).
   rewrite /VALspec_range (big_sepL_lookup_acc _ _ (Z.to_nat (a - l.2))).
   2: { apply lookup_seq; split; eauto; lia. }
   iDestruct "H" as "[H _]".
@@ -731,7 +412,17 @@ Proof.
   iDestruct "H" as (?) "H".
   replace (l.2 + Z.to_nat (a - l.2)) with a by lia.
   iDestruct (mapsto_lookup with "Hm H") as %(? & ? & _ & _ & Hacc); iPureIntro.
-  rewrite /access_cohere /access_at /= perm_of_freeable -mem_lemmas.po_oo // in Hacc.
+  rewrite /access_cohere /access_at /= H // in Hacc.
+Qed.
+
+Lemma VALspec_range_can_free: forall m n l,
+  mem_auth m ∗ VALspec_range n Share.top l ⊢
+  ⌜∃ m', free m l.1 l.2 (l.2 + n) = Some m'⌝.
+Proof.
+  intros.
+  rewrite VALspec_range_perm; last apply perm_of_freeable.
+  apply bi.pure_mono; intros.
+  apply range_perm_free in H as [??]; eauto.
 Qed.
 
 Lemma mapsto_can_free: forall m ch v l,
@@ -764,212 +455,5 @@ Proof.
   rewrite address_mapsto_VALspec_range Hch.
   apply VALspec_range_free; done.
 Qed.
-
-(*
-Lemma writable_writable_after_alloc' : forall m1 m2 lo hi b lev loc IOK1 IOK2,
-  alloc m1 lo hi = (m2, b) ->
-  writable loc (m_phi (initial_mem m1 lev IOK1)) ->
-  writable loc (m_phi (initial_mem m2 lev IOK2)).
-Proof.
-intros.
-hnf in *.
-case_eq (m_phi (initial_mem m1 lev IOK1) @ loc); intros.
-rewrite H1 in H0.
-inv H0.
-rewrite H1 in H0.
-assert (~adr_range (b,lo) (hi-lo) loc). {
- assert (Ha := juicy_mem_access (initial_mem m1 lev IOK1) loc).
-  destruct loc. simpl in *.
-  rewrite H1 in Ha.
-  destruct H0 as [_ H0]. destruct k; inv H0.
-  intro Contra.
-  destruct Contra.
-  subst.
-  assert (access_at m1 (nextblock m1, z) Cur = None).
-    unfold access_at; apply nextblock_noaccess; simpl. apply Plt_strict.
-  assert (b0 = nextblock m1) by (eapply alloc_result; eauto).
-  subst.
-  rewrite Ha in H0. simpl in H0. clear - r H0.
-  unfold perm_of_sh in H0. repeat if_tac in H0; try contradiction; inv H0.
-}
-apply alloc_dry_unchanged_on with (m1:=m1)(m2:=m2) in H2; auto.
-destruct H2.
-unfold initial_mem; simpl.
-unfold inflate_initial_mem, inflate_initial_mem'.
-rewrite resource_at_make_rmap.
-destruct loc as (b',ofs').
-assert (Ha := juicy_mem_access (initial_mem m1 lev IOK1) (b',ofs')). {
-  rewrite H1 in Ha.
-  destruct H0 as [Hfree H0]. destruct k; try solve [inversion H0].
-  unfold perm_of_res in Ha. simpl in Ha.
-  rewrite <- H3.
-  rewrite <- H2. rewrite Ha.
-  clear - Hfree r.
-  unfold perm_of_sh. rewrite if_true by auto. if_tac; auto.
-  rewrite Ha. unfold perm_of_sh. rewrite if_true by auto. 
-  clear; if_tac; congruence.
- }
- rewrite H1 in H0. simpl in H0. contradiction.
-Qed.
-
-Lemma readable_eq_after_alloc' : forall m1 m2 lo hi b lev loc IOK1 IOK2,
-  alloc m1 lo hi = (m2, b) ->
-  readable loc (m_phi (initial_mem m1 lev IOK1)) ->
-  m_phi (initial_mem m1 lev IOK1) @ loc=m_phi (initial_mem m2 lev IOK2) @ loc.
-Proof.
-intros.
-hnf in H0.
-case_eq (m_phi (initial_mem m1 lev IOK1) @ loc); intros.
-rewrite H1 in H0.
-inv H0.
-rewrite H1 in H0.
-assert (~adr_range (b,lo) (hi-lo) loc). {
- assert (Ha := juicy_mem_access (initial_mem m1 lev IOK1) loc).
-  destruct loc. simpl in *.
-  rewrite H1 in Ha.
-  destruct k; try solve [inv H0].
-  intro Contra.
-  destruct Contra.
-  subst.
-  assert (b0 = nextblock m1) by (eapply alloc_result; eauto).
-  subst.
-  simpl in Ha.
-(*
-  destruct (perm_of_sh_pshare t p) as [p' H4].
-  unfold perm_of_res in Ha; simpl in Ha; rewrite H4 in Ha.
-*)
-  assert (access_at m1 (nextblock m1, z) Cur = None).
-    unfold access_at. simpl. apply nextblock_noaccess. apply Plt_strict.
-  rewrite H2 in Ha.
-  clear - Ha r. unfold perm_of_sh in Ha. repeat if_tac in Ha; inv Ha; try contradiction.
-}
-apply alloc_dry_unchanged_on with (m1:=m1)(m2:=m2) in H2; auto.
-destruct H2.
-rewrite <- H1.
-unfold initial_mem; simpl.
-unfold inflate_initial_mem, inflate_initial_mem'.
-do 2 rewrite resource_at_make_rmap.
-destruct loc as (b',ofs').
- assert (Ha := juicy_mem_access (initial_mem m1 lev IOK1) (b',ofs')). {
-   rewrite H1 in Ha.   unfold perm_of_res in Ha; simpl in Ha.
-   simpl in H0. destruct k; try contradiction.
-  rewrite <- H2. rewrite Ha in *.
-  spec H3. clear - r. unfold perm_of_sh. repeat if_tac; try congruence; contradiction.
-  rewrite <- H3.
-  unfold perm_of_sh. if_tac. if_tac; auto. rewrite if_true by auto. auto.
-
- }
- rewrite H1 in H0. contradiction.
-Qed.
-
-Lemma perm_order''_trans p1 p2 p3 :
-  perm_order'' p1 p2 ->
-  perm_order'' p2 p3 ->
-  perm_order'' p1 p3.
-Proof.
-  destruct p1, p2, p3; simpl; try tauto.
-  apply perm_order_trans.
-Qed.
-
-Lemma po_join_sub_sh sh1 sh2 :
-  join_sub sh2 sh1 ->
-  Mem.perm_order'' (perm_of_sh sh1) (perm_of_sh sh2).
-Proof.
-  intros [sh J].
-  unfold perm_of_sh.
-  if_tac. if_tac. repeat if_tac; constructor.
-  if_tac. rewrite if_false. constructor.
-  contradict H0. subst. apply join_top in J; auto.
-  repeat if_tac; constructor.
-  assert (~writable0_share sh2) by (contradict H; eapply join_writable01; eauto).
-  if_tac. rewrite if_false by auto. repeat if_tac; constructor.
-  rewrite (if_false (writable0_share sh2)) by auto.
-  assert (~readable_share sh2) by (contradict H1; eapply join_readable1; eauto).
-  rewrite (if_false (readable_share sh2)) by auto.
-  if_tac.
-  subst. apply split_identity in J. apply identity_share_bot in J.
-  rewrite if_true by auto. constructor.
-  auto. if_tac; constructor.
-Qed.
-
-Lemma po_join_sub r1 r2 :
-  join_sub r2 r1 ->
-  Mem.perm_order'' (perm_of_res r1) (perm_of_res r2).
-Proof.
-  intros. destruct H as [r J]. inv J; simpl.
-  if_tac. subst. apply split_identity in RJ.
-  apply identity_share_bot in RJ. rewrite if_true by auto; constructor.
-  auto. if_tac; constructor.
-  destruct k; try constructor; apply po_join_sub_sh; eexists; eauto.
-  apply perm_order''_trans with (Some Nonempty).
-  destruct k; try constructor.
-  unfold perm_of_sh. if_tac. if_tac; constructor. rewrite if_true by auto; constructor.
-  if_tac; constructor.
-  destruct k; try constructor. apply po_join_sub_sh; eexists; eauto.
-  constructor.
-Qed.
-
-(*
-Lemma po_join_sub' r1 r2 :
-  join_sub r2 r1 ->
-  Mem.perm_order'' (perm_of_res' r1) (perm_of_res' r2).
-Proof.
-  
-*)
-Lemma perm_of_res_lock_not_Freeable:
-  forall r,
-    perm_order'' (Some Writable) (perm_of_res_lock r).
-Proof.
-  intros.
-  unfold perm_of_res_lock.
-  destruct r; try constructor.
-  destruct k; try constructor.
-  unfold perm_of_sh.
-  if_tac. rewrite if_false. constructor.
-  apply glb_Rsh_not_top.
-  repeat if_tac; constructor.
-Qed.
-
-Definition readable_perm (p: option permission) :
-  {perm_order'' p (Some Readable)}+{~perm_order'' p (Some Readable)}.
-destruct p.
-destruct p; try solve [left; constructor].
-all: right; intro; inv H.
-Defined.
-
-Definition rebuild_juicy_mem_fmap (jm: juicy_mem) (m': mem) : (AV.address -> resource) :=
- fun loc =>
-   match m_phi jm @ loc with
-    PURE k pp => PURE k pp
-   | NO sh rsh => if readable_perm (access_at m' loc Cur)
-                            then YES Tsh (writable_readable writable_share_top)
-                                        (VAL (contents_at m' loc)) NoneP
-                            else NO sh rsh 
-   | YES sh rsh (VAL _) _ => 
-                 if readable_perm (access_at m' loc Cur)
-                 then YES sh rsh (VAL (contents_at m' loc)) NoneP
-                 else NO _ bot_unreadable
-   | YES sh rsh _ _ => m_phi jm @ loc
-end.
-
-Definition rebuild_juicy_mem_rmap (jm: juicy_mem) (m': mem) :
-  {phi : rmap |
-  level phi = level jm /\
-  resource_at phi = rebuild_juicy_mem_fmap jm m' /\
-  ghost_of phi = ghost_of (m_phi jm)}.
-  refine (make_rmap (rebuild_juicy_mem_fmap jm m') (ghost_of (m_phi jm)) (level jm) _ _).
-extensionality loc.
-unfold compose.
-unfold rebuild_juicy_mem_fmap.
-destruct (m_phi jm @ loc) eqn:?H.
-if_tac; auto.
-pose proof (resource_at_approx (m_phi jm) loc).
-rewrite H in H0. simpl in H0.
-destruct k; simpl; auto.
-if_tac; auto.
-pose proof (resource_at_approx (m_phi jm) loc).
-rewrite H in *; auto.
-apply ghost_of_approx.
-Defined.*)
 
 End mpred.
